\solution 
From the given information, 
\begin{align}
% 
    a &= m+n,\\
    b &= n+p, \\
    c &= m+p 
\end{align}
which can be expressed as
\begin{align}
\myvec{1&1&0\\0&1&1\\1&0&1\\}\myvec{m\\n\\p} &= \myvec{a\\b\\c}
\\
\implies 
	\myvec{m\\n\\p} &= \myvec{1&1&0\\0&1&1\\1&0&1\\}^{-1}\myvec{a\\b\\c}
\end{align}
Using row reduction,
		\begin{align}
			\augvec{3}{3}{1&1&0 & 1 & 0 & 0\\0&1&1 & 0 & 1 & 0\\1&0&1 & 0 & 0 & 1}
			\xleftrightarrow[]{R_3 \leftarrow R_3 - R_1}
			\augvec{3}{3}{1&1&0 & 1 & 0 & 0\\0&1&1 & 0 & 1 & 0\\0&-1&1 & -1 & 0 & 1}
		\end{align}
		\begin{align}
			\xleftrightarrow[R_1 \leftarrow R_1 - R_2]{R_3 \leftarrow R_3 + R_2}
			\augvec{3}{3}{1&0&-1 & 1 & -1 & 0\\0&1&1 & 0 & 1 & 0\\0&0&2 & -1 & 1 & 1}
		\end{align}
		\begin{align}
			\xleftrightarrow[R_1 \leftarrow 2R_1 + R_3]{R_2 \leftarrow 2R_2 - R_3}
			\augvec{3}{3}{2&0&0 & 1 & -1 & 1\\0&2&0 & 1 & 1 & -1\\0&0&2 & -1 & 1 & 1}
		\end{align}
yielding
		\begin{align}
			\myvec{1&1&0\\0&1&1\\1&0&1\\}^{-1} = 
			\frac{1}{2}\myvec{1 & -1 & 1\\ 1 & 1 & -1\\ -1 & 1 & 1}
		\end{align}
	Therefore,
\begin{align}
\begin{split}
    p&=\frac{c+b-a}{2}
    =\frac{\sqrt{74}+\sqrt{32}-\sqrt{122}}{2}
    \\
    m&=\frac{a+c-b}{2}
    =\frac{\sqrt{74}+\sqrt{122}-\sqrt{32}}{2}
    \\
    n&=\frac{a+b-c}{2}
    =\frac{\sqrt{122}+\sqrt{32}-\sqrt{74}}{2}
\end{split}
	\label{eq:incircle-mnp}
\end{align}
upon substituting from 
		\eqref{eq:geo-norm-ab},
		\eqref{eq:geo-norm-bc}
		and
		\eqref{eq:geo-norm-ca}.
