\begin{enumerate}
	\item Since,
\begin{align}
\vec{A}-\vec{B} &= \myvec{5\\-7}, \\
	\norm{\vec{A}-\vec{B}} &= \sqrt{\myvec{5 & -7}\myvec{5\\-7}}
= \sqrt{\brak{5}^2 +\brak{7}^2}\\
	&=\sqrt{74}
		\label{eq:geo-norm-ab}
\end{align}
	\item Similarly, 
\begin{align}
\vec{B}-\vec{C} &= \myvec{-1\\11}\\
\implies 
\norm{\vec{B}-\vec{C}} &= \sqrt{\myvec{-1 & 11}\myvec{-1\\11}}
= \sqrt{\brak{1}^2+\brak{11}^2}
\\
	&= \sqrt{122}
		\label{eq:geo-norm-bc}
\end{align}
and
	\item \begin{align}
\vec{A}-\vec{C} &= \myvec{4\\4}\\
\implies
\norm{\vec{A}-\vec{C}} &= \sqrt{\myvec{4 & 4}\myvec{4\\4}}
= \sqrt{\brak{4}^2+\brak{4}^2}
\\
	&=\sqrt{32}
		\label{eq:geo-norm-ca}
\end{align}
\end{enumerate}
